README.md
@@ -15,7 +15,7 @@ I am currently working on Vol 1: LF.
 | Logic | √ |
 | IndProp | √ |
 | Maps | √ |
-| Imp | 40% |
+| Imp | √ |
 | ... | X |
 
 
